src/datalog/TypedDatalog.v
@@ -1,0 +1,295 @@
+From Stdlib Require Import Arith.Arith.
+From Stdlib Require Import Lists.List.
+From Stdlib Require Import micromega.Lia.
+From Stdlib Require Import Permutation.
+From Stdlib Require Import Classical_Prop.
+
+From coqutil Require Import Map.Interface Map.Properties Map.Solver Tactics Tactics.fwd Datatypes.List Datatypes.Option Eqb.
+
+From Datalog Require Import Map Tactics Fp List Eqb DotNotation Datalog.
+From GraphSearch Require Import Dag.
+
+Import ListNotations.
+
+Class type_signature {rel fn aggregator : Type} : Type :=
+  {
+    type : Type;
+    fun_type : fn -> list type * type;
+    rel_type : rel -> list type;
+    agg_type : aggregator -> type * type;
+  }.
+Arguments type_signature : clear implicits.
+
+Section __.
+  Context {rel : relT} {exprvar : exprvarT} {fn : fnT} {aggregator : aggregatorT}.
+  Context {var_eqb : Eqb exprvar} {var_eqb_ok : Eqb_ok var_eqb}.
+  Context `{tsig : type_signature rel fn aggregator}.
+  Context {type_context : map.map exprvar type}
+          {type_context_ok : map.ok type_context}.
+
+  Unset Elimination Schemes.
+  Inductive well_typed_expr (tctx : type_context) : expr -> type -> Prop :=
+  | wt_var_expr x t :
+    map.get tctx x = Some t ->
+    well_typed_expr tctx (expr.var x) t
+  | wt_fun_expr f args arg_ts t :
+    fun_type f = (arg_ts, t) ->
+    Forall2 (well_typed_expr tctx) args arg_ts ->
+    well_typed_expr tctx (expr.app f args) t.
+  Set Elimination Schemes.
+
+  Definition well_typed_clause (tctx : type_context) (c : clause) : Prop :=
+    Forall2 (well_typed_expr tctx) c.{args} (rel_type c.{rel}).
+
+  Definition well_typed_opt_expr (tctx : type_context) (oe : option expr) (t : type) : Prop :=
+    match oe with
+    | None => True
+    | Some e => well_typed_expr tctx e t
+    end.
+
+  Definition well_typed_meta_clause (tctx : type_context) (c : meta_clause) : Prop :=
+    Forall2 (well_typed_opt_expr tctx)
+      c.{args} (rel_type c.{rel}).
+
+  Definition well_typed_rule (r : rule) : Prop :=
+    exists tctx : type_context,
+      match r with
+      | normal_rule concls hyps =>
+          Forall (well_typed_clause tctx) concls /\
+          Forall (well_typed_clause tctx) hyps
+      | meta_rule concls hyps =>
+          Forall (well_typed_meta_clause tctx) concls /\
+          Forall (well_typed_meta_clause tctx) hyps
+      | agg_rule concl_rel agg hyp_rel =>
+          exists i_type in_type out_type shared,
+            agg_type agg = (in_type, out_type) /\
+            rel_type concl_rel = out_type :: shared /\
+            rel_type hyp_rel = i_type :: in_type :: shared
+      end.
+
+  Context {type_eqb : Eqb type} {type_eqb_ok : Eqb_ok type_eqb}.
+
+  Fixpoint check_expr_type e t : option type_context :=
+    match e with
+    | expr.var x => Some (map.put map.empty x t)
+    | expr.app f args =>
+        let '(arg_ts, ret_t) := fun_type f in
+        if (type_eqb ret_t t && Nat.eqb (length arg_ts) (length args))%bool
+        then compatible_union_of_list_option (map2 check_expr_type args arg_ts)
+        else None
+    end.
+
+  Definition check_clause_type (c : clause) : option type_context :=
+    let arg_ts := rel_type c.{rel} in
+    if Nat.eqb (length c.{args}) (length arg_ts)
+    then compatible_union_of_list_option
+           (map2 check_expr_type c.{args} arg_ts)
+    else None.
+
+  Definition check_opt_expr_type (oe : option expr) (t : type) : option type_context :=
+    match oe with
+    | None => Some map.empty
+    | Some e => check_expr_type e t
+    end.
+
+  Definition check_meta_clause_type (c : meta_clause) : option type_context :=
+    let arg_ts := rel_type c.{rel} in
+    if Nat.eqb (length c.{args}) (length arg_ts)
+    then compatible_union_of_list_option
+           (map2 check_opt_expr_type c.{args} arg_ts)
+    else None.
+
+  Definition check_rule_type (r : rule) : option type_context :=
+    match r with
+    | normal_rule concls hyps =>
+        compatible_union_of_list_option
+         
+          (map check_clause_type (concls ++ hyps))
+    | meta_rule concls hyps =>
+        compatible_union_of_list_option
+         
+          (map check_meta_clause_type (concls ++ hyps))
+    | agg_rule concl_rel agg hyp_rel =>
+        let '(in_type, out_type) := agg_type agg in
+        match rel_type concl_rel, rel_type hyp_rel with
+        | out_t :: c_shared, _ :: in_t :: h_shared =>
+            if (type_eqb out_type out_t &&
+                type_eqb in_type in_t &&
+                list_eqb c_shared h_shared)%bool
+            then Some map.empty
+            else None
+        | _, _ => None
+        end
+    end.
+
+  Lemma well_typed_expr_extends e :
+    forall tctx tctx' t,
+      well_typed_expr tctx e t ->
+      map.extends tctx' tctx ->
+      well_typed_expr tctx' e t.
+  Proof.
+    induction e; intros tctx tctx' t' Hwt Hext.
+    - inversion Hwt; subst. constructor. apply Hext. assumption.
+    - inversion Hwt; subst. econstructor; [eassumption|].
+      eapply Forall2_impl_strong; [eassumption|].
+      intros a t_a Hwa Hin _. rewrite Forall_forall in H. eauto.
+  Qed.
+
+  Lemma well_typed_clause_extends tctx tctx' c :
+    well_typed_clause tctx c ->
+    map.extends tctx' tctx ->
+    well_typed_clause tctx' c.
+  Proof.
+    cbv [well_typed_clause]. intros H Hext.
+    eapply Forall2_impl_strong; [eassumption|].
+    intros; eauto using well_typed_expr_extends.
+  Qed.
+
+  Lemma well_typed_meta_clause_extends tctx tctx' c :
+    well_typed_meta_clause tctx c ->
+    map.extends tctx' tctx ->
+    well_typed_meta_clause tctx' c.
+  Proof.
+    cbv [well_typed_meta_clause]. intros H Hext.
+    eapply Forall2_impl_strong; [eassumption|].
+    intros [e|] t Hopt _ _; cbv [well_typed_opt_expr] in *;
+      eauto using well_typed_expr_extends.
+  Qed.
+
+  Lemma check_expr_type_sound e :
+    forall t tctx,
+      check_expr_type e t = Some tctx ->
+      well_typed_expr tctx e t.
+  Proof.
+    induction e; intros t' tctx Hck; simpl in Hck.
+    - injection Hck as <-.
+      constructor. apply map.get_put_same.
+    - destruct (fun_type f) as [arg_ts ret_t] eqn:Eft.
+      destruct ((type_eqb ret_t t' && Nat.eqb (length arg_ts) (length args))%bool) eqn:Echk;
+        [|discriminate].
+      apply Bool.andb_true_iff in Echk. destruct Echk as [Eret Elen].
+      destr (type_eqb ret_t t'); [|discriminate].
+      apply Nat.eqb_eq in Elen.
+      cbv [compatible_union_of_list_option] in Hck.
+      destruct (option_all (map2 check_expr_type args arg_ts)) as [ctxs|] eqn:Eall;
+        [|discriminate].
+      simpl in Hck.
+      destruct (compatible_union_of_list ctxs) as [u|] eqn:Eun;
+        [|discriminate].
+      simpl in Hck. injection Hck as <-.
+      apply option_all_map2_Forall3 in Eall; [|congruence].
+      econstructor; [eassumption|].
+      pose proof (compatible_union_of_list_extends _ _ Eun) as Hext.
+      apply Forall3_ignore3_strong in Eall.
+      eapply Forall2_impl_strong; [eassumption|].
+      intros a t_a [c [Hin Hck_a]] Hin_a _.
+      rewrite Forall_forall in H.
+      eapply well_typed_expr_extends; eauto.
+  Qed.
+
+  Lemma check_clause_type_sound c tctx :
+    check_clause_type c = Some tctx ->
+    well_typed_clause tctx c.
+  Proof.
+    cbv [check_clause_type well_typed_clause].
+    destruct (Nat.eqb (length c.{args}) (length (rel_type c.{rel})))
+      eqn:Elen; [|discriminate].
+    apply Nat.eqb_eq in Elen.
+    intros Hck.
+    cbv [compatible_union_of_list_option] in Hck.
+    destruct (option_all (map2 check_expr_type c.{args} (rel_type c.{rel})))
+      as [ctxs|] eqn:Eall; [|discriminate].
+    simpl in Hck.
+    destruct (compatible_union_of_list ctxs) as [u|] eqn:Eun;
+      [|discriminate].
+    simpl in Hck. injection Hck as <-.
+    apply option_all_map2_Forall3 in Eall; [|assumption].
+    pose proof (compatible_union_of_list_extends _ _ Eun) as Hext.
+    apply Forall3_ignore3_strong in Eall.
+    eapply Forall2_impl_strong; [eassumption|].
+    intros a t_a [c0 [Hin Hck_a]] _ _.
+    eapply well_typed_expr_extends; eauto using check_expr_type_sound.
+  Qed.
+
+  Lemma check_meta_clause_type_sound c tctx :
+    check_meta_clause_type c = Some tctx ->
+    well_typed_meta_clause tctx c.
+  Proof.
+    cbv [check_meta_clause_type well_typed_meta_clause].
+    destruct (Nat.eqb (length c.{args}) (length (rel_type c.{rel})))
+      eqn:Elen; [|discriminate].
+    apply Nat.eqb_eq in Elen.
+    intros Hck.
+    cbv [compatible_union_of_list_option] in Hck.
+    destruct (option_all (map2 check_opt_expr_type c.{args} (rel_type c.{rel})))
+      as [ctxs|] eqn:Eall; [|discriminate].
+    simpl in Hck.
+    destruct (compatible_union_of_list ctxs) as [u|] eqn:Eun;
+      [|discriminate].
+    simpl in Hck. injection Hck as <-.
+    apply option_all_map2_Forall3 in Eall; [|assumption].
+    pose proof (compatible_union_of_list_extends _ _ Eun) as Hext.
+    apply Forall3_ignore3_strong in Eall.
+    eapply Forall2_impl_strong; [eassumption|].
+    intros [e|] t_a [c0 [Hin Hck_a]] _ _;
+      cbv [check_opt_expr_type well_typed_opt_expr] in *.
+    - eapply well_typed_expr_extends; eauto using check_expr_type_sound.
+    - exact I.
+  Qed.
+
+  Lemma check_rule_type_sound r tctx :
+    check_rule_type r = Some tctx ->
+    well_typed_rule r.
+  Proof.
+    cbv [check_rule_type well_typed_rule]. destruct r as [concls hyps|concls hyps|cr ag hr].
+    - intros Hck. exists tctx.
+      cbv [compatible_union_of_list_option] in Hck.
+      destruct (option_all (map check_clause_type (concls ++ hyps))) as [ctxs|] eqn:Eall;
+        [|discriminate].
+      simpl in Hck.
+      destruct (compatible_union_of_list ctxs) as [u|] eqn:Eun;
+        [|discriminate].
+      simpl in Hck. inversion Hck; subst u; clear Hck.
+      pose proof (compatible_union_of_list_extends _ _ Eun) as Hext.
+      apply option_all_map_Some' in Eall.
+      apply Forall_app.
+      enough (Hall : Forall (well_typed_clause tctx) (concls ++ hyps)) by tauto.
+      apply Forall_forall. intros c0 Hin.
+      assert (In (check_clause_type c0) (map Some ctxs)) as Hin'
+          by (rewrite <- Eall; apply in_map; assumption).
+      apply in_map_iff in Hin'. destruct Hin' as [m [Heq Hin_m]].
+      eapply well_typed_clause_extends; [eauto using check_clause_type_sound|].
+      auto.
+    - intros Hck. exists tctx.
+      cbv [compatible_union_of_list_option] in Hck.
+      destruct (option_all (map check_meta_clause_type (concls ++ hyps))) as [ctxs|] eqn:Eall;
+        [|discriminate].
+      simpl in Hck.
+      destruct (compatible_union_of_list ctxs) as [u|] eqn:Eun;
+        [|discriminate].
+      simpl in Hck. inversion Hck; subst u; clear Hck.
+      pose proof (compatible_union_of_list_extends _ _ Eun) as Hext.
+      apply option_all_map_Some' in Eall.
+      apply Forall_app.
+      enough (Hall : Forall (well_typed_meta_clause tctx) (concls ++ hyps)) by tauto.
+      apply Forall_forall. intros c0 Hin.
+      assert (In (check_meta_clause_type c0) (map Some ctxs)) as Hin'
+          by (rewrite <- Eall; apply in_map; assumption).
+      apply in_map_iff in Hin'. destruct Hin' as [m [Heq Hin_m]].
+      eapply well_typed_meta_clause_extends;
+        [eauto using check_meta_clause_type_sound|]. auto.
+    - destruct (agg_type ag) as [in_t out_t] eqn:Eagt.
+      destruct (rel_type cr) as [|out_t' c_sh] eqn:Ecr; [discriminate|].
+      destruct (rel_type hr) as [|i_t [|in_t' h_sh]] eqn:Ehr; try discriminate.
+      destruct ((type_eqb out_t out_t' &&
+                 type_eqb in_t in_t' &&
+                 list_eqb c_sh h_sh)%bool) eqn:Echk; [|discriminate].
+      intros _.
+      apply Bool.andb_true_iff in Echk. destruct Echk as [Echk Esh].
+      apply Bool.andb_true_iff in Echk. destruct Echk as [Eout Ein].
+      destr (type_eqb out_t out_t'); [|discriminate].
+      destr (type_eqb in_t in_t'); [|discriminate].
+      destr (list_eqb c_sh h_sh); [|discriminate].
+      exists map.empty, i_t, in_t', out_t', h_sh. auto.
+  Qed.
+End __.
